WIP invariant and partial proofs for SHA-256 padder (#921)

silveroak-opentitan/hmac/hw/Sha256Properties.v
@@ -21,6 +21,7 @@ Require Import Coq.ZArith.ZArith.
 Require Import Coq.Init.Byte.
 Require Import Coq.Lists.List.
 Require Import coqutil.Tactics.Tactics.
+Require Import Cava.Util.BitArithmetic.
 Require Import Cava.Util.If.
 Require Import Cava.Util.List.
 Require Import Cava.Util.Nat.
@@ -251,3 +252,391 @@ Proof.
         repeat destruct_one_match_hyp; f_equal; lia).
   cbn [fst snd]. push_resize. reflexivity.
 Qed.
+
+(* values of padder state constants *)
+Definition padder_waiting_value : N := 0.
+Definition padder_emit_bit_value : N := 1.
+Definition padder_flushing_value : N := 2.
+Definition padder_writing_length_value : N := 3.
+
+(* Correctness for padder state constant circuits *)
+Lemma step_padder_waiting : step padder_waiting tt tt = (tt, padder_waiting_value).
+Proof. reflexivity. Qed.
+Hint Rewrite @step_padder_waiting using solve [eauto] : stepsimpl.
+Lemma step_padder_emit_bit : step padder_emit_bit tt tt = (tt, padder_emit_bit_value).
+Proof. reflexivity. Qed.
+Hint Rewrite @step_padder_emit_bit using solve [eauto] : stepsimpl.
+Lemma step_padder_flushing : step padder_flushing tt tt = (tt, padder_flushing_value).
+Proof. reflexivity. Qed.
+Hint Rewrite @step_padder_flushing using solve [eauto] : stepsimpl.
+Lemma step_padder_writing_length :
+  step padder_writing_length tt tt = (tt, padder_writing_length_value).
+Proof. reflexivity. Qed.
+Hint Rewrite @step_padder_writing_length using solve [eauto] : stepsimpl.
+
+Definition expected_padder_state
+           (msg : list Byte.byte) (msg_complete : bool) (i : nat) : N :=
+  if msg_complete
+  then if i =? length msg
+       then padder_emit_bit_value
+       else
+         (* check if message ends early enough for length to fit in same
+            block (block=64 bytes, length=8 bytes, 64-8=56) *)
+         if (length msg + 1) mod 64 <? 56
+         then if 56 <=? i mod 64
+              then padder_writing_length_value
+              else padder_flushing_value
+         else if i <? length msg + 8
+              then padder_flushing_value
+              else if 56 <=? i mod 64
+                   then padder_writing_length_value
+                   else padder_flushing_value
+  else padder_waiting_value.
+
+(* State invariant for sha256_padder *)
+Definition sha256_padder_invariant
+           (state : denote_type (Bit ** sha_word ** Bit ** BitVec 4 ** BitVec 61 ** BitVec 16))
+           (msg : list Byte.byte) (msg_complete padder_done : bool) (index : nat) : Prop :=
+  let '(done, (out, (out_valid, (state, (len, current_offset))))) := state in
+  (* index is always a multiple of 4 *)
+  index mod 4 = 0
+  (* ...and length matches the length of the message so far in bytes *)
+  /\ len = N.of_nat (length msg)
+  (* ...and offset is always in the range [0,15] *)
+  /\ (0 <= current_offset < 16)%N
+  (* ...and the [padder_done] ghost variable just tracks [done] *)
+  /\ done = padder_done
+  /\ (if out_valid
+     then
+       (* if output is valid, we must have processed at least one word *)
+       4 <= index
+       (* ...and the output must match the spec *)
+       /\ out = BigEndianBytes.concat_bytes
+                 (firstn 4 (skipn (index - 4) (SHA256.padded_msg_bytes msg)))
+     else True)
+  /\ (if done
+     then
+       (* if we're done, we must be in the padder_waiting state *)
+       state = padder_waiting_value
+       (* ...and if the output is valid, the index must be at the end of the
+          expected result *)
+       /\ (if out_valid
+          then index = length (SHA256.padded_msg_bytes msg)
+          else index = 0 /\ msg = [])
+     else
+       (* if we're not done, the word index must be in range *)
+       index < length (SHA256.padded_msg_bytes msg)
+       (* ...and the current offset matches index *)
+       /\ (current_offset * 4 = N.of_nat index mod 64)%N
+       (* ...and the state must match the message and word index *)
+       /\ state = expected_padder_state msg msg_complete index).
+
+(* Precondition for sha256_padder *)
+Definition sha256_padder_pre
+           (input : denote_type [Bit; BitVec 32; Bit; BitVec 4; Bit; Bit])
+           (msg : list Byte.byte) (msg_complete padder_done : bool) (index : nat) : Prop :=
+  let '(data_valid, (data, (is_final, (final_length, (consumer_ready, (clear,_)))))) := input in
+  (* message length, plus any new data, must be small enough that size in bits
+     fits in a 64-bit word *)
+  (if data_valid
+   then if is_final
+        then (N.of_nat (length msg) + final_length < 2 ^ 61)%N
+        else (N.of_nat (length msg) + 4 < 2 ^ 61)%N
+   else (N.of_nat (length msg) < 2 ^ 61)%N)
+  (* ...and if clear is true, then the message ghost variable is empty *)
+  /\ (if clear then msg = [] /\ index = 0 else True)
+  /\ (if data_valid
+     then
+       (* caller is only allowed to pass new valid data if we're in the
+          padder_waiting state *)
+       expected_padder_state msg msg_complete index = padder_waiting_value
+       (* ...and the message is complete iff is_final is true *)
+       /\ msg_complete = is_final
+       /\ (if is_final
+          then
+            (* if this is the final word, and the message must have
+               [final_length] additional bytes beyond what was already
+               processed *)
+            length msg = index + N.to_nat final_length
+            (* ...and final_length must be in the range [1,4] *)
+            /\ 1 <= N.to_nat final_length <= 4
+          else
+            (* if this is not the final word, the message must have exactly 4
+               additional bytes beyond what was already processed *)
+            length msg = index + 4)
+     else
+       (* is_final must be false if data is not valid *)
+       is_final = false
+    ).
+
+Definition sha256_padder_spec
+           (input : denote_type [Bit; BitVec 32; Bit; BitVec 4; Bit; Bit])
+           (state : denote_type (Bit ** sha_word ** Bit ** BitVec 4 ** BitVec 61 ** BitVec 16))
+           (msg : list Byte.byte) (msg_complete padder_done : bool) (index : nat)
+  : denote_type (Bit ** sha_word ** Bit) :=
+  let '(data_valid, (data, (is_final, (final_length, (consumer_ready, (clear,_)))))) := input in
+  let '(done, (out, (out_valid, (state, (len, current_offset))))) := state in
+  (* expected result as words *)
+  let expected_words := SHA256.padded_msg msg in
+  let word_index := index / 4 in
+  let out_valid :=
+      if clear
+      then false
+      else if consumer_ready
+           then if padder_done
+                then data_valid (* we were previously done and got new valid data *)
+                else 0 <? word_index (* we're partway through processing message *)
+           else false (* dummy output if consumer is not ready *) in
+  let out :=
+      if clear
+      then 0%N
+      else if consumer_ready
+           then nth word_index expected_words 0%N (* output matches expected value *)
+           else 0%N (* dummy output if consumer is not ready *) in
+  let done :=
+      if clear
+      then true
+      else if consumer_ready
+           then
+             (* either this was the last word, or we were previously done and didn't
+                start a new message this step *)
+             ((word_index =? length expected_words - 1)
+              || (done && negb data_valid))%bool
+           else done (* stay in same state if consumer not ready *) in
+  (out_valid, (out, done)).
+
+(* TODO: move *)
+Lemma step_bvresize {n m} (x : denote_type (BitVec n)) :
+  step (bvresize (n:=n) m) tt (x, tt) = (tt, N.land x (N.ones (N.of_nat m))).
+Proof. reflexivity. Qed.
+Hint Rewrite @step_bvresize using solve [eauto] : stepsimpl.
+
+(* TODO: move *)
+Lemma length_N_to_bytes n bs :
+  length (BigEndianBytes.N_to_bytes n bs) = n.
+Admitted.
+Hint Rewrite @length_N_to_bytes : push_length.
+(* TODO: move *)
+Lemma length_bytes_to_Ns_upper_bound n bs :
+  length (BigEndianBytes.bytes_to_Ns n bs) * n < length bs + n.
+Admitted.
+(* TODO: move *)
+Lemma padded_message_bytes_longer_than_input msg :
+  length msg < length (SHA256.padded_msg_bytes msg).
+Admitted.
+Lemma padded_message_longer_than_input msg :
+  length (BigEndianBytes.bytes_to_Ns 4 msg) < length (SHA256.padded_msg msg).
+Admitted.
+(* TODO: move *)
+Lemma padded_message_bytes_min_length msg :
+  64 <= length (SHA256.padded_msg_bytes msg).
+Admitted.
+(* TODO: move *)
+Lemma padded_message_min_length msg : 16 <= length (SHA256.padded_msg msg).
+Admitted.
+(* TODO: move *)
+(* Adding data cannot decrease padded message size *)
+Lemma padded_message_bytes_length_mono msg data :
+  length (SHA256.padded_msg_bytes msg) <=
+  length (SHA256.padded_msg_bytes (msg ++ data)).
+Admitted.
+
+(* Shorthand to calculate the new value of the [index] ghost variable for the
+   padder *)
+Definition padder_update_index
+           (msg : list Byte.byte) (msg_complete padder_done : bool) (index : nat)
+           (input : denote_type [Bit; BitVec 32; Bit; BitVec 4; Bit; Bit])
+  : nat :=
+  let '(data_valid, (data, (is_final, (final_length, (consumer_ready, (clear,_)))))) := input in
+  if clear
+  then 0
+  else if consumer_ready
+       then if padder_done
+            then if data_valid
+                 then 4
+                 else 0
+            else if msg_complete
+                 then index + 4
+                 else if data_valid
+                      then index + 4
+                      else index
+       else index.
+
+(* Shorthand to calculate the new value of the [msg] ghost variable for the
+   padder *)
+Definition padder_update_msg
+           (msg : list Byte.byte) (msg_complete padder_done : bool) (index : nat)
+           (input : denote_type [Bit; BitVec 32; Bit; BitVec 4; Bit; Bit])
+  : list Byte.byte :=
+  let '(data_valid, (data, (is_final, (final_length, (consumer_ready, (clear,_)))))) := input in
+  if clear
+  then []
+  else if consumer_ready
+       then if padder_done
+            then if data_valid
+                 then BigEndianBytes.N_to_bytes 4 data
+                 else []
+            else if data_valid
+                 then msg ++ BigEndianBytes.N_to_bytes 4 data
+                 else msg
+       else msg.
+
+(* Shorthand to calculate the new value of the [msg_complete] ghost variable for the
+   padder *)
+Definition padder_update_msg_complete
+           (msg : list Byte.byte) (msg_complete padder_done : bool) (index : nat)
+           (input : denote_type [Bit; BitVec 32; Bit; BitVec 4; Bit; Bit])
+  : bool :=
+  let '(data_valid, (data, (is_final, (final_length, (consumer_ready, (clear,_)))))) := input in
+  if clear
+  then false
+  else if consumer_ready
+       then if data_valid
+            then is_final
+            else msg_complete
+       else msg_complete.
+
+(* Shorthand to calculate the new value of the [padder_done] ghost variable for the
+   padder *)
+Definition padder_update_padder_done
+           (msg : list Byte.byte) (msg_complete padder_done : bool) (index : nat)
+           (input : denote_type [Bit; BitVec 32; Bit; BitVec 4; Bit; Bit])
+  : bool :=
+  let '(data_valid, (data, (is_final, (final_length, (consumer_ready, (clear,_)))))) := input in
+  let new_index := padder_update_index msg msg_complete padder_done index input in
+  let new_msg := padder_update_msg msg msg_complete padder_done index input in
+  if clear
+  then true
+  else if consumer_ready
+       then if padder_done
+            then negb data_valid
+            else new_index =? length (SHA256.padded_msg_bytes new_msg)
+       else padder_done.
+
+Lemma step_sha256_padder_invariant input state msg msg_complete padder_done index :
+  sha256_padder_pre input msg msg_complete padder_done index ->
+  sha256_padder_invariant state msg msg_complete padder_done index ->
+  sha256_padder_invariant
+    (fst (step sha256_padder state input))
+    (padder_update_msg msg msg_complete padder_done index input)
+    (padder_update_msg_complete msg msg_complete padder_done index input)
+    (padder_update_padder_done msg msg_complete padder_done index input)
+    (padder_update_index msg msg_complete padder_done index input).
+Proof.
+  (* keep track of the values of input and state so they're visible as we
+     destruct cases; helps to figure out what case you're in when
+     writing/debugging proofs *)
+  pose (I:=input). pose (S:=state). pose (mc:=msg_complete).
+  destruct input as
+      (data_valid, (data, (is_final, (final_length, (consumer_ready, (clear,[])))))).
+  destruct state as
+      (done, (out, (out_valid, (state, (len, current_offset))))).
+  (* simplify single-step behavior *)
+  cbv [sha256_padder_pre sha256_padder_invariant
+                         padder_update_msg
+                         padder_update_msg_complete
+                         padder_update_padder_done
+                         padder_update_index].
+  intros. logical_simplify. subst. cbn [fst snd] in *.
+  cbv [sha256_padder K]. stepsimpl.
+  repeat (destruct_pair_let; cbn [fst snd]).
+  autorewrite with tuple_if; cbn [fst snd].
+  stepsimpl.
+  (* destruct cases for flags *)
+  destruct clear;
+    repeat (boolsimpl || subst || logical_simplify);
+    (* handle case for clear=true *)
+    [ ssplit; (lia || reflexivity || (cbn; tauto)) | ].
+  destruct consumer_ready;
+    repeat (boolsimpl || subst || logical_simplify);
+    rewrite ?N.eqb_refl;
+    (* handle case for consumer_ready=false *)
+    [ | ssplit; (lia || reflexivity || (cbn; tauto)) ].
+  destruct data_valid;
+    repeat (boolsimpl || subst || logical_simplify);
+    cbn [N.eqb Pos.eqb padder_waiting_value padder_flushing_value
+               padder_emit_bit_value padder_writing_length_value].
+  { (* Case for handling valid data:
+       consumer_ready=true
+       clear=false
+       data_valid=true
+     *)
+    pose proof length_bytes_to_Ns_upper_bound 4 msg.
+    pose proof padded_message_longer_than_input msg.
+    pose proof padded_message_bytes_longer_than_input msg.
+    pose proof padded_message_bytes_min_length msg.
+    let data := lazymatch goal with |- context [msg ++ ?data] => data end in
+    pose proof padded_message_bytes_length_mono msg data;
+    pose proof padded_message_bytes_min_length data.
+    ssplit.
+    { (* index is a multiple of 4 *)
+      repeat destruct_one_match;
+        rewrite ?Nat.mod_add with (b:=1) (c:=4); auto. }
+    { (* length matches length processed so far *)
+      rewrite N.land_ones.
+      rewrite N.add_mod_idemp_r by (cbn;lia).
+      compute_expr (2 ^ N.of_nat 61)%N.
+      lazymatch goal with H : context [(2 ^ 61)%N] |- _ => cbn in H end.
+      cbv [expected_padder_state] in *.
+      destruct is_final; logical_simplify; subst; boolsimpl.
+      all:repeat (destruct_one_match_hyp; try discriminate).
+      all:logical_simplify; subst; cbn [length app] in *.
+      all:rewrite ?N.eqb_refl; try lia.
+      all:push_length.
+      all:rewrite N.mod_small; lia. }
+    { (* offset stays in range *)
+      change (2 ^ N.of_nat 4)%N with 16%N.
+      apply N.mod_bound_pos; lia. }
+    { (* offset stays in range *)
+      change (2 ^ N.of_nat 4)%N with 16%N.
+      apply N.mod_bound_pos; lia. }
+    { (* padder_done matches done *)
+      repeat destruct_one_match; [ reflexivity | | ];
+      logical_simplify; subst.
+      all:symmetry; apply Nat.eqb_neq.
+      all:let data := lazymatch goal with |- context [?msg ++ ?data] => data end in
+          pose proof padded_message_bytes_longer_than_input (msg ++ data).
+      all:autorewrite with push_length in *; lia. }
+    { (* if output is valid, then new index must be at least 4 *)
+      repeat destruct_one_match; lia. }
+    { (* output matches spec *)
+      admit. }
+    { cbv [expected_padder_state] in *.
+      destruct padder_done, out_valid, is_final; logical_simplify; subst.
+      all:repeat (destruct_one_match_hyp; try discriminate).
+      all:repeat destruct_one_match; lia. }
+    { (* new offset matches expectations *)
+      cbv [expected_padder_state] in *. change (2 ^ N.of_nat 4)%N with 16%N.
+      destruct padder_done, out_valid, is_final; logical_simplify; subst.
+      all:repeat (destruct_one_match_hyp; try discriminate).
+      all:cbn [length app] in *.
+      all:repeat destruct_one_match; try lia.
+      all:admit.
+      (* modular arithmetic, proof sketch:
+         Given: offset * 4 = index mod 64
+         Prove: (offset + 1) mod 16 * 4 = (index + 4) mod 64
+
+         (index + 4) mod 64 (RHS)
+         = (index mod 64 + 4) mod 64
+         = (offset * 4 + 4) mod 64
+         = ((offset + 1) * 4) mod 64
+         (now easier to think in terms of bitwise representations)
+         = ((offset + 1) << 2) & N.ones 6
+         = ((offset + 1) & N.ones 4) << 2
+         (back to numeric)
+         = (offset + 1) mod 16 * 4 (LHS)
+       *)
+    }
+    { (* new state matches expectation *)
+      cbv [expected_padder_state] in *.
+      destruct padder_done, out_valid, is_final;
+        logical_simplify; subst; rewrite ?N.eqb_refl; boolsimpl.
+      all:repeat (destruct_one_match_hyp; try discriminate).
+      all:repeat destruct_one_match; try discriminate; reflexivity. } }
+  { (* Case for handling invalid data:
+       consumer_ready=true
+       clear=false
+       data_valid=false
+     *)
+    admit. }
+Admitted.
